new_trusted_code/github_com/goose_lang/goose/machine.v
@@ -2,3 +2,4 @@
 From New.code Require Import github_com.goose_lang.primitive.
 
 Module machine := primitive.
+Export machine.
