src/goose_lang/ffi/disk_ffi/adequacy.v
@@ -2,7 +2,6 @@ From stdpp Require Import gmap.
 From stdpp Require Import vector fin_maps.
 
 From Perennial.goose_lang Require Import lang lifting.
-From Perennial.goose_lang.lib Require Import slice.
 
 From Perennial.goose_lang.ffi.disk_ffi Require Import impl specs.
 
@@ -13,7 +12,7 @@ From Perennial.goose_lang Require Import adequacy.
 
 #[global]
 Program Instance disk_interp_adequacy:
-  @ffi_interp_adequacy disk.disk_model disk_interp disk.disk_op disk.disk_semantics :=
+  @ffi_interp_adequacy disk_model disk_interp disk_op disk_semantics :=
   {| ffiGpreS := disk_preG;
      ffiΣ := diskΣ;
      subG_ffiPreG := subG_diskG;
@@ -35,8 +34,8 @@ Next Obligation.
 Qed.
 
 Section crash.
-  Existing Instances disk.disk_op disk.disk_model disk.disk_ty.
-  Existing Instances disk.disk_semantics disk_interp.
+  Existing Instances disk_op disk_model.
+  Existing Instances disk_semantics disk_interp.
   Existing Instance goose_diskGS.
 
   Lemma disk_pointsto_post_crash `{!heapGS Σ} l q v:
