src/goose_lang/ffi/disk_ffi/typed_impl.v
@@ -1,0 +1,61 @@
+From Perennial.goose_lang Require Export ffi.disk_ffi.impl.
+From Perennial.goose_lang Require Export lang notation typing.
+From Perennial.goose_lang.lib Require Export slice.
+
+Inductive Disk_ty := | DiskInterfaceTy.
+
+#[global]
+Instance disk_val_ty: val_types :=
+  {| ext_tys := Disk_ty; |}.
+
+Inductive disk_ext_tys : @val disk_op -> (ty * ty) -> Prop :=
+| DiskOpType op :
+  disk_ext_tys (λ: "v", ExternalOp op (Var "v"))%V
+    (match op with
+     | ReadOp => (uint64T, arrayT byteT)
+     | WriteOp => (prodT uint64T (arrayT byteT), unitT)
+     | SizeOp => (unitT, uint64T)
+     end).
+
+Definition disk_ty : ext_types disk_op :=
+  {| val_tys := disk_val_ty;
+    get_ext_tys := disk_ext_tys |}.
+
+Module disk.
+  Definition Disk: ty := extT DiskInterfaceTy.
+
+  (** * Disk user-facing operations. *)
+  (* these are local instances on purpose, so that importing this files doesn't
+  suddenly cause all FFI parameters to be inferred as the disk model *)
+  Existing Instances disk_op disk_model disk_ty.
+
+  Definition disk_val (d : ()) : val := ExtV d.
+
+  Definition blockT `{ext_tys:ext_types}: @ty val_tys := slice.T byteT.
+
+  Definition BlockSize := BlockSize.
+
+  Definition Get: val :=
+    λ: <>, disk_val ().
+
+  Definition Read: val :=
+    λ: "a",
+    let: "p" := ExternalOp ReadOp (Var "a") in
+    raw_slice byteT (Var "p") #4096.
+
+  Definition ReadTo: val :=
+    λ: "a" "buf",
+    let: "p" := ExternalOp ReadOp (Var "a") in
+    MemCpy_rec byteT (slice.ptr (Var "buf")) (Var "p") #4096.
+
+  Definition Write: val :=
+    λ: "a" "b",
+    ExternalOp WriteOp (Var "a", slice.ptr (Var "b")).
+
+  Definition Barrier: val :=
+    λ: <>, #().
+
+  Definition Size: val :=
+    λ: "v",
+       ExternalOp SizeOp (Var "v").
+End disk.
