src/goose_lang/ffi/disk_prelude.v
@@ -1,10 +1,10 @@
 From Perennial.goose_lang Require Import lang.
-From Perennial.goose_lang Require ffi.disk_ffi.impl.
+From Perennial.goose_lang Require Export ffi.disk_ffi.typed_impl.
 From Perennial.goose_lang Require Export ffi.disk.
 #[global]
-Existing Instances disk.disk_op disk.disk_model disk.disk_ty.
+Existing Instances disk_op disk_model disk_ty.
 #[global]
-Existing Instances disk.disk_semantics disk_interp.
+Existing Instances disk_semantics disk_interp.
 #[global]
 Existing Instance goose_diskGS.
 (* Now that the TC parameter is fixed, we can make this a coercion. Sadly,
